@@ -1,0 +1,45 @@
+module
+
+public import Roolean.QfBv.BvTerm
+public import Roolean.SmtLib2.Lexer
+public import Roolean.SmtLib2.Proof
+
+public inductive Proof.Node (v: VarWidths)
+  | Relevant
+  | Irrelevant
+  | Split (varIndex: Fin v.size) (bitIndex: Fin (v.varWidth varIndex))
+    (left: Proof.Node v) (right: Proof.Node v)
+deriving Repr
+
+public structure Proof (v: VarWidths) where
+  result: Bool
+  root: Proof.Node v
+
+namespace Proof
+
+public inductive EOfSmt
+  | BadVarIndex
+  | BadBitIndex
+deriving Repr
+
+public def Node.ofSmt (n: SmtNode) (v: VarWidths) : Except EOfSmt (Node v) := do
+  match n with
+  | .Relevant => pure Node.Relevant
+  | .Irrelevant => pure Node.Irrelevant
+  | .Split varIndex bitIndex left right =>
+    if hVarIndex: varIndex < v.size then
+      let varIndex := Fin.mk varIndex hVarIndex
+      if hBitIndex: bitIndex < v.varWidth varIndex then
+        let bitIndex := (Fin.mk bitIndex hBitIndex)
+        let left ← Node.ofSmt left v
+        let right ← Node.ofSmt right v
+        pure (Node.Split varIndex bitIndex left right)
+
+      else
+        Except.error EOfSmt.BadBitIndex
+    else
+      Except.error EOfSmt.BadVarIndex
+
+public def ofSmt (proof: SmtProof) (v: VarWidths) : Except EOfSmt (Proof v) := do
+  let root ← Node.ofSmt proof.root v
+  pure { result := proof.result, root }
